complete library

test.hs
@@ -1,0 +1,107 @@
+
+
+module Test where
+
+import qualified Prelude
+
+__ :: any
+__ = Prelude.error "Logical or arity value used"
+
+data Bool =
+   True
+ | False
+
+data Nat =
+   O
+ | S Nat
+
+nat_rect :: a1 -> (Nat -> a1 -> a1) -> Nat -> a1
+nat_rect f f0 n =
+  case n of {
+   O -> f;
+   S n0 -> f0 n0 (nat_rect f f0 n0)}
+
+nat_rec :: a1 -> (Nat -> a1 -> a1) -> Nat -> a1
+nat_rec =
+  nat_rect
+
+data Sum a b =
+   Inl a
+ | Inr b
+
+type Sig a =
+  a
+  -- singleton inductive, whose constructor was exist
+  
+append :: char list -> char list -> char list
+append s1 s2 =
+  case s1 of {
+   [] -> s2;
+   (::) c s1' -> (::) c (append s1' s2)}
+
+type Decidable = Sum () ()
+
+decidable_le_nat :: Nat -> Nat -> Decidable
+decidable_le_nat x =
+  nat_rec (\y -> Inl __) (\x0 iHx y ->
+    nat_rec (Inr __) (\y0 iHy ->
+      case iHx y0 of {
+       Inl _ -> Inl __;
+       Inr _ -> Inr __}) y) x
+
+type Showable a =
+  a -> char list
+  -- singleton inductive, whose constructor was Build_Showable
+  
+show :: (Showable a1) -> a1 -> char list
+show showable =
+  showable
+
+show_nat :: Showable Nat
+show_nat n =
+  nat_rec ((::)
+    ((* If this appears, you're using Ascii internals. Please don't *)
+ (fun (b0,b1,b2,b3,b4,b5,b6,b7) ->
+  let f b i = if b then 1 lsl i else 0 in
+  Char.chr (f b0 0 + f b1 1 + f b2 2 + f b3 3 + f b4 4 + f b5 5 + f b6 6 + f b7 7))
+    False False False False True True False False) []) (\n0 iHn ->
+    append ((::)
+      ((* If this appears, you're using Ascii internals. Please don't *)
+ (fun (b0,b1,b2,b3,b4,b5,b6,b7) ->
+  let f b i = if b then 1 lsl i else 0 in
+  Char.chr (f b0 0 + f b1 1 + f b2 2 + f b3 3 + f b4 4 + f b5 5 + f b6 6 + f b7 7))
+      True True False False True False True False) ((::)
+      ((* If this appears, you're using Ascii internals. Please don't *)
+ (fun (b0,b1,b2,b3,b4,b5,b6,b7) ->
+  let f b i = if b then 1 lsl i else 0 in
+  Char.chr (f b0 0 + f b1 1 + f b2 2 + f b3 3 + f b4 4 + f b5 5 + f b6 6 + f b7 7))
+      False False False False False True False False) ((::)
+      ((* If this appears, you're using Ascii internals. Please don't *)
+ (fun (b0,b1,b2,b3,b4,b5,b6,b7) ->
+  let f b i = if b then 1 lsl i else 0 in
+  Char.chr (f b0 0 + f b1 1 + f b2 2 + f b3 3 + f b4 4 + f b5 5 + f b6 6 + f b7 7))
+      False False False True False True False False) [])))
+      (append iHn ((::)
+        ((* If this appears, you're using Ascii internals. Please don't *)
+ (fun (b0,b1,b2,b3,b4,b5,b6,b7) ->
+  let f b i = if b then 1 lsl i else 0 in
+  Char.chr (f b0 0 + f b1 1 + f b2 2 + f b3 3 + f b4 4 + f b5 5 + f b6 6 + f b7 7))
+        True False False True False True False False) []))) n
+
+failed_cast :: a1 -> char list -> a1
+failed_cast = Prelude.error "Cast has failed"
+
+cast :: (Showable a1) -> (a1 -> Decidable) -> a1 -> a1
+cast h dec a =
+  case dec a of {
+   Inl _ -> a;
+   Inr _ -> failed_cast a (show h a)}
+
+g :: Nat -> Nat
+g x =
+  S O
+
+client :: Nat -> Nat
+client x =
+  g (cast show_nat (decidable_le_nat (S O)) x)
+
