test.ml
@@ -1,0 +1,75 @@
+type __ = Obj.t
+let __ = let rec f _ = Obj.repr f in Obj.repr f
+
+type bool =
+| True
+| False
+
+type nat =
+| O
+| S of nat
+
+type ('a, 'b) sum =
+| Inl of 'a
+| Inr of 'b
+
+type 'a sig0 =
+  'a
+  (* singleton inductive, whose constructor was exist *)
+
+(** val append : char list -> char list -> char list **)
+
+let rec append s1 s2 =
+  match s1 with
+  | [] -> s2
+  | c::s1' -> c::(append s1' s2)
+
+type decidable = (__, __) sum
+
+(** val decidable_le_nat : nat -> nat -> decidable **)
+
+let rec decidable_le_nat n y =
+  match n with
+  | O -> Inl __
+  | S n0 ->
+    (match y with
+     | O -> Inr __
+     | S n1 ->
+       (match decidable_le_nat n0 n1 with
+        | Inl _ -> Inl __
+        | Inr _ -> Inr __))
+
+type 'a showable =
+  'a -> char list
+  (* singleton inductive, whose constructor was Build_Showable *)
+
+(** val show : 'a1 showable -> 'a1 -> char list **)
+
+let show showable0 =
+  showable0
+
+(** val show_nat : nat showable **)
+
+let rec show_nat = function
+| O -> '0'::[]
+| S n0 -> append ('S'::(' '::('('::[]))) (append (show_nat n0) (')'::[]))
+
+(** val cast : 'a1 showable -> ('a1 -> decidable) -> 'a1 -> 'a1 **)
+
+let cast h dec a =
+  match dec a with
+  | Inl _ -> a
+  | Inr _ ->
+    (let f _ s = failwith (String.concat "" (["Cast has failed because of "]@ (List.map (String.make 1) s))) in f)
+      a (show h a)
+
+(** val g : nat -> nat **)
+
+let g x =
+  S O
+
+(** val client : nat -> nat **)
+
+let client x =
+  g (cast show_nat (decidable_le_nat (S O)) x)
+
