test.mli
@@ -1,0 +1,40 @@
+
+
+type __ = Obj.t
+
+type bool =
+| True
+| False
+
+type nat =
+| O
+| S of nat
+
+type ('a, 'b) sum =
+| Inl of 'a
+| Inr of 'b
+
+type 'a sig0 =
+  'a
+  (* singleton inductive, whose constructor was exist *)
+
+val append : char list -> char list -> char list
+
+type decidable = (__, __) sum
+
+val decidable_le_nat : nat -> nat -> decidable
+
+type 'a showable =
+  'a -> char list
+  (* singleton inductive, whose constructor was Build_Showable *)
+
+val show : 'a1 showable -> 'a1 -> char list
+
+val show_nat : nat showable
+
+val cast : 'a1 showable -> ('a1 -> decidable) -> 'a1 -> 'a1
+
+val g : nat -> nat
+
+val client : nat -> nat
+
