Cast.v
@@ -1,61 +1,64 @@
 Require Export Unicode.Utf8_core.
-
-Require Export DecidableExtns.
+Add LoadPath "." as Casts.
+Require Import String Decidable Showable.
 
 Notation "x .1" := (proj1_sig x) (at level 3).
 Notation "x .2" := (proj2_sig x) (at level 3).
 Notation " ( x ; p ) " := (exist _ x p).
 
-Axiom failed_cast : forall {A:Type} {P : A -> Prop} (a: A) (msg:Prop), {a : A | P a}.
-  
-Definition cast (A:Type) (P : A -> Prop) 
-  (dec : forall a, Decidable (P a)) : A -> {a : A | P a}.
-Proof.
-  intro a. case (dec a); intro p.
-  - exact (a; p).
-  - exact (failed_cast a (P a)).
-Defined.
+Axiom failed_cast : 
+  forall {A:Type} {P : A -> Prop} (a:A) {msg1:string} (msg2: Prop), {a : A | P a}.
+
+Definition cast (A:Type) `{Showable A} (P : A -> Prop) 
+  (dec : forall a, Decidable (P a)) : A -> {a : A | P a} :=
+fun a: A => 
+  match dec a with
+    | inl p => (a ; p)
+    | inr _ => failed_cast a (msg1 := show a) (P a)
+  end.
+
 Notation "?" := (cast _ _ _).
 
-Definition cast_fun_range (A B : Type) (P : B -> Prop) 
+Definition cast_fun_range (A B : Type) `{Showable B} (P : B -> Prop) 
   (dec : forall b, Decidable (P b)) :
     (A -> B) -> A -> {b : B | P b} :=
   fun f a => ? (f a).
 Notation "?>" := (cast_fun_range _ _ _ _).
 
-Definition cast_fun_dom (A B : Type) (P: A -> Prop) 
+Definition cast_fun_dom (A B : Type) `{Showable A} (P: A -> Prop) 
   (dec: forall a, Decidable (P a)) :
     ({a : A | P a} -> B)  -> A -> B :=
   fun f a => f (? a).
 Notation "<?" := (cast_fun_dom _ _ _ _).
 
-Definition cast_forall_range (A: Type) (B: A -> Type) 
+
+Definition cast_forall_range (A: Type) (B: A -> Type) `{forall a, Showable (B a)}
   (P : forall a:A, B a -> Prop) 
   (dec : forall a (b : B a), Decidable (P a b)) :
     (forall a: A, B a) -> forall a: A, {b : B a | P a b} :=
   fun f a => ? (f a).
-Notation "?>>" := (cast_forall_range _ _ _ _).
-
-Axiom failed_cast_type : forall {A:Type} {P : A -> Prop} {a: A} (msg:Prop),
- (failed_cast (P:=P) a msg).1 = a.
+Notation "??>" := (cast_forall_range _ _ _ _).
 
 
-Definition hide_cast (A: Type) (P: A -> Prop) (B: A -> Type)
+Axiom failed_cast_type : 
+  forall {A:Type} `{Showable A} {P : A -> Prop} {a: A} (msg:Prop),
+    (failed_cast (P:=P) a (msg1 := show a) msg).1 = a.
+
+Definition hide_cast (A: Type) (P: A -> Prop) (B: A -> Type) `{Showable A}
            (dec: forall a, Decidable (P a)) (a:A): B (? a).1 -> B a.
 Proof.
   unfold cast. case (dec a); intro p.
   - exact (fun b => b).
   - exact (fun b => eq_rect _ _ b _ (failed_cast_type (P a))).
 Defined.
+
 Notation "[?]" := (hide_cast _ _ _ _ _).
 
 
-Definition cast_forall_dom (A: Type) (P: A -> Prop) 
+Definition cast_forall_dom (A: Type) (P: A -> Prop) `{Showable A}
            (B: A -> Type) (dec: forall a, Decidable (P a)) :
    (forall x: {a : A | P a}, B x.1)  -> (forall a : A, B a) :=
   fun f a => [?] (f (? a)).
-Notation "<<?" := (cast_forall_dom _ _ _ _).
+Notation "<??" := (cast_forall_dom _ _ _ _).
 
-Require Import List.
-Definition cast_list A (P : A -> Prop) (_ : forall a, Decidable (P a))  : list A -> list {a : A | P a} := map ?.
-Notation "?::" := (cast_list _ _). 
+
