Showable.v
@@ -1,0 +1,12 @@
+Require Import String. 
+
+Class Showable (A :Type) := { show : A -> string }.
+
+Local Open Scope string_scope.
+
+Instance show_nat : Showable nat.
+econstructor. intro n ; induction n.
+exact "0". exact ("S ("++IHn++")").
+Defined.
+
+Definition not_implemented := "not implemented".
