records.v
@@ -1,0 +1,96 @@
+Require Export Unicode.Utf8_core.
+Add LoadPath "." as Casts.
+Require Import Cast Decidable Showable.
+Require Import Nat Arith.
+Require Import Eqdep_dec.
+Require Import Arith.
+
+Definition bnat (n:nat) := {m : nat | m <= n}.
+
+Definition bnat_to_nat n : bnat n -> nat := fun x => x.1.
+
+Coercion bnat_to_nat : bnat >-> nat.
+
+Instance show_bnat k : Showable (bnat k) := {| show := fun n => show n.1|}.
+
+Record Rat : Set := mkRat
+   {sign : bool;
+    top : nat;
+    bottom : nat;
+    Rat_bottom_cond : 0 <> bottom;
+    Rat_irred_cond : forall x y z: bnat (max top bottom),
+        x * y = top /\ x * z = bottom -> 1 = x}.
+
+Definition bnat_S n : bnat n -> bnat (S n) :=
+  fun m => (m.1; le_S _ _ m.2).
+
+(* Adapted from https://coq.inria.fr/files/interval_discr.v *)
+
+Theorem eq_rect_eq_nat :
+  forall (p:nat) (Q:nat->Type) (x:Q p) (h:p=p), x = eq_rect p Q x p h.
+Proof.
+intros. apply K_dec_set with (p := h). apply eq_nat_dec. reflexivity.
+Qed.
+
+Scheme le_ind' := Induction for le Sort Prop.
+
+Definition le_hprop : forall (n m : nat) (p q : n <= m), p = q.
+Proof.
+induction p using le_ind'; intro q.
+- replace (le_n n) with
+  (eq_rect _ (fun n0 => n <= n0) (le_n n) _ eq_refl) by reflexivity.
+  generalize (eq_refl n). case q.
+  + intro e. rewrite <- eq_rect_eq_nat. reflexivity.
+  + intros m l e. contradiction (le_Sn_n m); rewrite <- e; assumption.
+- replace (le_S n m p) with
+  (eq_rect _ (fun n0 => n <= n0) (le_S n m p) _ eq_refl) by reflexivity.
+  generalize (eq_refl (S m)). case q.
+  + intro Heq. contradiction (le_Sn_n m); rewrite Heq; assumption.
+  + intros m0 l HeqS. injection HeqS; intro Heq; generalize l HeqS.
+    rewrite <- Heq; intros; rewrite <- eq_rect_eq_nat.
+    rewrite (IHp l0); reflexivity.
+Qed.
+
+Fixpoint _Decidable_forall_bounded k (P: bnat k-> Prop)
+         (HP : forall n, Decidable (P n)) {struct k}:
+  Decidable (forall n : bnat k, P n).
+destruct k.
+- case (HP (0;Le.le_O_n _)); intro H.
+  + left. destruct n. destruct (Le.le_n_0_eq _ l).
+    rewrite (le_hprop 0 0 l (Le.le_O_n _)). exact H.
+  + right. intro H0. apply (H ([?] (H0 _))).
+- case (_Decidable_forall_bounded k (fun n => P (bnat_S k n))
+                                   (fun n => HP (bnat_S k n))); intro H.
+  + case (HP (S k; Le.le_refl _)). intro HPk.
+    * left. intro n. destruct n as [n Hn]. inversion Hn; subst.
+      rewrite (le_hprop _ _ Hn (Le.le_refl _)). exact HPk.
+      rewrite (le_hprop _ _ Hn (le_S _ _ H1)). exact (H (n;H1)). 
+    * right. intro H0. apply n. exact (H0 (S k; Le.le_refl _)).
+  + right. intro H0. apply H. intro n. exact (H0 (bnat_S _ n)).
+Defined.
+
+Instance Decidable_forall_bounded k
+  (P:bnat k->Prop) (HP : forall n, Decidable (P n)) :
+  Decidable (forall n, P n).
+exact (_Decidable_forall_bounded _ _ _). Defined.
+
+
+
+Axiom failed_cast_Rat : forall (s:bool) (t b: nat), Rat.
+
+Definition cast_Rat (s:bool) (t b: nat) : Rat :=
+  match dec _ (*Rat_bottom_cond*), dec _ (*Rat_irred_cond*) with
+    | inl Hb , inl Hi => mkRat s t b Hb Hi
+    | _ , _ => failed_cast_Rat s t b
+  end.
+
+Axiom failed_cast_top : forall s t b, top (failed_cast_Rat s t b) = t.
+
+Definition Rat_good := cast_Rat true 5 6.
+
+Eval compute in top Rat_good.
+
+Definition Rat_bad := cast_Rat true 5 10.
+
+Eval compute in top Rat_bad.
+
