Makefile
@@ -1,0 +1,16 @@
+COQDOCOPTS=--utf8 -g --interpolate --body-only -R . Casts -coqlib http://coq.inria.fr/stdlib/ 
+COQOPTS=
+COQBIN=
+
+all: coqcompile ${TARGETS} 
+
+coqcompile:
+	coq_makefile -R . Casts *.v -o Makefile_coq
+	$(MAKE) -f Makefile_coq > \dev\null
+
+%.vo: %.v
+	${COQBIN}coqc ${COQOPTS} $<
+
+clean: 
+	$(MAKE) -f Makefile_coq clean
+	rm -f ${TARGETS}
